Significant progress on implementing Spec.HPKE

specs/experimental/Spec.HPKE.CFRG.fst
@@ -20,44 +20,6 @@ let pow2_35_less_than_pow2_125 : _:unit{pow2 32 * pow2 3 <= pow2 125 - 1} = asse
 
 #set-options "--z3rlimit 200"
 
-/// Types
-
-let is_ciphersuite = function
-  | DH.DH_Curve25519, AEAD.AEAD_AES128_GCM,        Hash.SHA2_256
-  | DH.DH_Curve25519, AEAD.AEAD_Chacha20_Poly1305, Hash.SHA2_256
-  | DH.DH_Curve448,   AEAD.AEAD_AES256_GCM,        Hash.SHA2_512
-  | DH.DH_Curve448,   AEAD.AEAD_Chacha20_Poly1305, Hash.SHA2_512
-  | DH.DH_P256,       AEAD.AEAD_AES128_GCM,        Hash.SHA2_256
-  | DH.DH_P256,       AEAD.AEAD_Chacha20_Poly1305, Hash.SHA2_256 -> true
-  | _,_,_ -> false
-
-type ciphersuite = cs:(DH.algorithm & AEAD.algorithm & Hash.algorithm){is_ciphersuite cs}
-
-
-inline_for_extraction
-let size_cs_identifier: size_nat = 1
-
-
-val id_of_cs: cs:ciphersuite -> Tot (lbytes size_cs_identifier)
-let id_of_cs cs =
-  match cs with
-  | DH.DH_Curve25519, AEAD.AEAD_AES128_GCM,        Hash.SHA2_256 -> create 1 (u8 1)
-  | DH.DH_Curve25519, AEAD.AEAD_Chacha20_Poly1305, Hash.SHA2_256 -> create 1 (u8 2)
-  | DH.DH_Curve448,   AEAD.AEAD_AES256_GCM,        Hash.SHA2_512 -> create 1 (u8 3)
-  | DH.DH_Curve448,   AEAD.AEAD_Chacha20_Poly1305, Hash.SHA2_512 -> create 1 (u8 4)
-  | DH.DH_P256,       AEAD.AEAD_AES128_GCM,        Hash.SHA2_256 -> create 1 (u8 5)
-  | DH.DH_P256,       AEAD.AEAD_Chacha20_Poly1305, Hash.SHA2_256 -> create 1 (u8 6)
-
-
-let curve_of_cs (cs:ciphersuite) : DH.algorithm =
-  let (c,a,h) = cs in c
-
-let aead_of_cs (cs:ciphersuite) : AEAD.algorithm =
-  let (c,a,h) = cs in a
-
-let hash_of_cs (cs:ciphersuite) : Hash.algorithm =
-  let (c,a,h) = cs in h
-
 
 /// Constants
 
@@ -85,6 +47,61 @@ let label_nonce : lbytes size_label_nonce = createL label_nonce_list
 let label_key : lbytes size_label_key = createL label_key_list
 
 
+/// Types
+
+inline_for_extraction
+let size_cs_identifier: size_nat = 2
+
+inline_for_extraction
+let size_mode_identifier: size_nat = 1
+
+
+let is_ciphersuite = function
+  | DH.DH_Curve25519, AEAD.AEAD_AES128_GCM,        Hash.SHA2_256
+  | DH.DH_Curve25519, AEAD.AEAD_Chacha20_Poly1305, Hash.SHA2_256
+  | DH.DH_Curve448,   AEAD.AEAD_AES256_GCM,        Hash.SHA2_512
+  | DH.DH_Curve448,   AEAD.AEAD_Chacha20_Poly1305, Hash.SHA2_512
+  | DH.DH_P256,       AEAD.AEAD_AES128_GCM,        Hash.SHA2_256
+  | DH.DH_P256,       AEAD.AEAD_Chacha20_Poly1305, Hash.SHA2_256 -> true
+  | _,_,_ -> false
+
+type ciphersuite = cs:(DH.algorithm & AEAD.algorithm & Hash.algorithm){is_ciphersuite cs}
+
+
+val id_of_cs: cs:ciphersuite -> Tot (lbytes size_cs_identifier)
+let id_of_cs cs =
+  match cs with
+  | DH.DH_Curve25519, AEAD.AEAD_AES128_GCM,        Hash.SHA2_256 -> create 2 (u8 1)
+  | DH.DH_Curve25519, AEAD.AEAD_Chacha20_Poly1305, Hash.SHA2_256 -> create 2 (u8 2)
+  | DH.DH_Curve448,   AEAD.AEAD_AES256_GCM,        Hash.SHA2_512 -> create 2 (u8 3)
+  | DH.DH_Curve448,   AEAD.AEAD_Chacha20_Poly1305, Hash.SHA2_512 -> create 2 (u8 4)
+  | DH.DH_P256,       AEAD.AEAD_AES128_GCM,        Hash.SHA2_256 -> create 2 (u8 5)
+  | DH.DH_P256,       AEAD.AEAD_Chacha20_Poly1305, Hash.SHA2_256 -> create 2 (u8 6)
+
+
+let curve_of_cs (cs:ciphersuite) : DH.algorithm =
+  let (c,a,h) = cs in c
+
+let aead_of_cs (cs:ciphersuite) : AEAD.algorithm =
+  let (c,a,h) = cs in a
+
+let hash_of_cs (cs:ciphersuite) : Hash.algorithm =
+  let (c,a,h) = cs in h
+
+
+type mode =
+  | Base
+  | PSK
+  | Auth
+  | PSKAuth
+
+val id_of_mode: m:mode -> Tot (lbytes size_mode_identifier)
+let id_of_mode m =
+  match m with
+  | Base -> create 1 (u8 0)
+  | PSK -> create 1 (u8 1)
+  | Auth -> create 1 (u8 2)
+  | PSKAuth -> create 1 (u8 3)
 
 /// Constants sizes
 
@@ -101,11 +118,26 @@ inline_for_extraction
 let size_dh_public (cs:ciphersuite): size_nat = DH.size_public (curve_of_cs cs)
 
 inline_for_extraction
-let size_einfo: size_nat = 32
+let size_kdf (cs:ciphersuite): size_nat = Hash.size_hash (hash_of_cs cs)
 
 inline_for_extraction
-let size_context (cs:ciphersuite): size_nat =
-  size_cs_identifier + 2 * size_dh_public cs + size_einfo
+let size_psk (cs:ciphersuite): size_nat = size_kdf cs
+
+
+
+(* inline_for_extraction *)
+(* let size_einfo: size_nat = 32 *)
+
+(* inline_for_extraction *)
+(* let size_context (cs:ciphersuite): size_nat = *)
+(*   size_cs_identifier + 2 * size_dh_public cs + size_einfo *)
+
+inline_for_extraction
+let max_pskID: size_nat = pow2 16 - 1
+
+inline_for_extraction
+let max_info: size_nat = pow2 16 - 1
+
 
 /// Types
 
@@ -113,133 +145,274 @@ type key_dh_public_s (cs:ciphersuite) = lbytes (size_dh_public cs)
 type key_dh_secret_s (cs:ciphersuite) = lbytes (size_dh_key cs)
 type key_aead_s (cs:ciphersuite) = lbytes (size_aead_key cs)
 type nonce_aead_s (cs:ciphersuite) = lbytes (size_aead_nonce cs)
+type psk_s (cs:ciphersuite) = lbytes (size_psk cs)
 
 
-
-val build_context:
-    cs:ciphersuite
-  -> key_dh_public_s cs
-  -> key_dh_public_s cs
-  -> lbytes (size_einfo) ->
-  Tot (lbytes (size_context cs))
-
-let build_context cs pkE pkR einfo =
-  let idcs: lbytes 1 = id_of_cs cs in
-  idcs @| pkE @| pkR @| einfo
-
-
-/// SetupI()
-///
-/// Input: ciphersuite, pkR, info
-///
-///    1. (skE, pkE) = GenerateKeyPair()
-///    2. zz = DH(skE, pkR)
-///    3. secret = Extract(0^Nh, zz)
-///    4. context = ciphersuite || Marshal(pkE) || Marshal(pkR) || info
-///    6. keyIR = Expand(secret, "hpke key" || context, Nk)
-///    8. nonceIR = Expand(secret, "hpke nonce" || context, Nn)
-///
-/// Output: pkE, keyIR, nonceIR
+/// def Encap(pkR):
+///     skE, pkE = GenerateKeyPair()
+///     zz = DH(skE, pkR)
+///     enc = Marshal(pkE)
+///     return zz, enc
 
 val encap:
     cs: ciphersuite
   -> skE: key_dh_secret_s cs
-  -> pkR: key_dh_public_s cs
-  -> einfo: lbytes size_einfo ->
-  Tot (key_dh_public_s cs & key_aead_s cs & nonce_aead_s cs)
+  -> pkR: key_dh_public_s cs ->
+  Tot (key_dh_public_s cs & key_dh_public_s cs)
 
-let encap cs skE pkR einfo =
+let encap cs skE pkR =
   let pkE = DH.secret_to_public (curve_of_cs cs) skE in
   let zz = DH.scalarmult (curve_of_cs cs) skE pkR in
-  let nh0 = create (size_dh_key cs) (u8 0) in
-  let secret = HKDF.extract (hash_of_cs cs) nh0 zz in
-  let context: lbytes (size_context cs) = build_context cs pkE pkR einfo in
-  let info_key: lbytes (size_context cs + size_label_key) = label_key @| context in
-  let info_nonce: lbytes (size_context cs + size_label_nonce) = label_nonce @| context in
-  let keyIR = HKDF.expand (hash_of_cs cs) secret info_key (size_aead_key cs) in
-  let nonceIR = HKDF.expand (hash_of_cs cs) secret info_nonce (size_aead_nonce cs) in
-  pkE, keyIR, nonceIR
+  zz, pkE
 
 
-/// SetupR()
-///
-/// Input: ciphersuite, pkE, skR, info
-///
-///    1. zz = DH(skR, pkE)
-///    2. secret = Extract(0^Nh, zz)
-///    3. context = ciphersuite || Marshal(pkE) || Marshal(pkR) || info
-///    4. keyIR = Expand(secret, "hpke key" || context, Nk)
-///    5. nonceIR = Expand(secret, "hpke nonce" || context, Nn)
-///
-/// Output: keyIR, nonceIR
+/// def Decap(enc, skR):
+///      pkE = Unmarshal(enc)
+///      return DH(skR, pkE)
 
 val decap:
     cs: ciphersuite
   -> pkE: key_dh_public_s cs
-  -> skR: key_dh_secret_s cs
-  -> einfo: lbytes size_einfo ->
+  -> skR: key_dh_secret_s cs ->
+  Tot (key_dh_public_s cs)
+
+let decap cs pkE skR = DH.scalarmult (curve_of_cs cs) skR pkE
+
+
+/// def AuthEncap(pkR, skI):
+///      skE, pkE = GenerateKeyPair()
+///      zz = concat(DH(skE, pkR), DH(skI, pkR))
+///      enc = Marshal(pkE)
+///      return zz, enc
+
+val auth_encap:
+    cs: ciphersuite
+  -> skE: key_dh_secret_s cs
+  -> skI: key_dh_secret_s cs
+  -> pkR: key_dh_public_s cs ->
+  Tot (lbytes (2 * size_dh_public cs) & key_dh_public_s cs)
+
+let auth_encap cs skE skI pkR =
+  let pkE = DH.secret_to_public (curve_of_cs cs) skE in
+  let er = DH.scalarmult (curve_of_cs cs) skE pkR in
+  let ir = DH.scalarmult (curve_of_cs cs) skI pkR in
+  let zz = concat er ir in
+  zz, pkE
+
+
+/// def AuthDecap(enc, skR, pkI):
+///      pkE = Unmarshal(enc)
+///      return concat(DH(skR, pkE), DH(skR, pkI))
+
+val auth_decap:
+    cs: ciphersuite
+  -> pkE: key_dh_public_s cs
+  -> pkI: key_dh_public_s cs
+  -> skR: key_dh_secret_s cs ->
+  Tot (lbytes (2 * size_dh_public cs))
+
+let auth_decap cs pkE pkI skR =
+  let re = DH.scalarmult (curve_of_cs cs) skR pkE in
+  let ri = DH.scalarmult (curve_of_cs cs) skR pkI in
+  concat re ri
+
+/// default_pkIm = zero(Npk)
+/// default_psk = zero(Nh)
+/// default_pskId = zero(0)
+
+let default_pkI (cs:ciphersuite):bytes = create (size_dh_public cs) (u8 0)
+let default_psk (cs:ciphersuite): bytes = create (size_psk cs) (u8 0)
+let default_pskId: b:bytes{Seq.length b = 0} = lbytes_empty
+
+
+/// def VerifyMode(mode, psk, pskID, pkIm):
+///     got_psk = (psk != default_psk and pskID != default_pskID)
+///     no_psk = (psk == default_psk and pskID == default_pskID)
+///     got_pkIm = (pkIm != default_pkIm)
+///     no_pkIm = (pkIm == default_pkIm)
+///
+///     if mode == mode_base and (got_psk or got_pkIm):
+///       raise Exception("Invalid configuration for mode_base")
+///     if mode == mode_psk and (no_psk or got_pkIm):
+///       raise Exception("Invalid configuration for mode_psk")
+///     if mode == mode_auth and (got_psk or no_pkIm):
+///       raise Exception("Invalid configuration for mode_auth")
+///     if mode == mode_psk_auth and (no_psk or no_pkIm):
+///       raise Exception("Invalid configuration for mode_psk_auth")
+///
+///
+/// BB. Implementing this function should not be necessary for us.
+///     We are filtering those using our option type in `ks_derive`.
+
+val build_context:
+    cs:ciphersuite
+  -> m:mode
+  -> pkE:key_dh_public_s cs
+  -> pkR:key_dh_public_s cs
+  -> pkI:key_dh_public_s cs
+  -> pskID:bytes{Seq.length pskID <= max_pskID}
+  -> info:bytes{Seq.length info <= max_pskID} ->
+  Tot bytes
+
+let build_context cs m pkE pkR pkI pskID info =
+  let pskID_len: lbytes 2 = nat_to_bytes_be 2 (Seq.length pskID) in
+  let info_len: lbytes 2 = nat_to_bytes_be 2 (Seq.length info) in
+  let context = (id_of_mode m) @| (id_of_cs cs) @| pkE @| pkR @| pkI in
+  let context = Seq.append context pskID_len in
+  let context = Seq.append context pskID in
+  let context = Seq.append context info_len in
+  let context = Seq.append context info in
+  context
+
+
+val ks_derive:
+    cs:ciphersuite
+  -> m:mode
+  -> pkR:key_dh_public_s cs
+  -> zz:bytes{Seq.length zz = size_dh_public cs \/ Seq.length zz = 2 * size_dh_public cs}
+  -> pkE:key_dh_public_s cs
+  -> info:bytes{Seq.length info <= max_info}
+  -> opsk:option (psk_s cs & id:bytes{Seq.length id <= max_pskID})
+  -> opkI:option (key_dh_public_s cs) ->
   Tot (key_aead_s cs & nonce_aead_s cs)
 
-let decap cs pkE skR einfo =
-  let pkR = DH.secret_to_public (curve_of_cs cs) skR in
-  let zz = DH.scalarmult (curve_of_cs cs) skR pkE in
-  let nh0 = create (size_dh_key cs) (u8 0) in
-  let secret = HKDF.extract (hash_of_cs cs) nh0 zz in
-  let context: lbytes (size_context cs) = build_context cs pkE pkR einfo in
-  let info_key: lbytes (size_context cs + size_label_key) = label_key @| context in
-  let info_nonce: lbytes (size_context cs + size_label_nonce) = label_nonce @| context in
+let ks_derive cs m pkR zz pkE info opsk opkI =
+  let (psk, pskID) =
+    match opsk with
+    | None -> (default_psk cs, default_pskId)
+    | Some (psk, pskID) -> (psk, pskID) in
+  let pkI =
+    match opkI with
+    | None -> default_pkI cs
+    | Some pki -> pki in
+  let context = build_context cs m pkE pkR pkI pskID info in
+  let secret = HKDF.extract (hash_of_cs cs) psk zz in
+  let info_key = Seq.append label_key context in
+  let info_nonce = Seq.append label_nonce context in
   let keyIR = HKDF.expand (hash_of_cs cs) secret info_key (size_aead_key cs) in
   let nonceIR = HKDF.expand (hash_of_cs cs) secret info_nonce (size_aead_nonce cs) in
   keyIR, nonceIR
 
 
-/// Encrypt()
-///
-/// Input: ciphersuite, pkR, info, ad, pt
-///
-///    1. pkE, keyIR, nonceIR = SetupI(ciphersuite, pkR, info)
-///    2. ct = Seal(keyIR, nonceIR, ad, pt)
-///
-/// Output: ct, pkE
+/// def SetupBaseI(pkR, info):
+///     zz, enc = Encap(pkR)
+///     return enc, KeySchedule(mode_base, pkR, zz, enc, info,
+///                             default_psk, default_pskID, default_pkIm)
 
-val encrypt:
-    cs: ciphersuite
+val setupBaseI:
+    cs:ciphersuite
   -> skE: key_dh_secret_s cs
-  -> pkR: key_dh_public_s cs
-  -> info: lbytes size_einfo
-  -> aad: bytes {length aad + AEAD.padlen (aead_of_cs cs) (length aad) <= max_size_t}
-  -> pt: bytes {length pt <= max_size_t
-           /\ length pt + AEAD.size_block (aead_of_cs cs) <= max_size_t
-           /\ length pt + AEAD.padlen (aead_of_cs cs) (length pt) <= max_size_t} ->
-  Tot (bytes & key_dh_public_s cs)
+  -> pkR:key_dh_public_s cs
+  -> info:bytes{Seq.length info <= max_info} ->
+  Tot (key_dh_public_s cs & key_aead_s cs & nonce_aead_s cs)
 
-let encrypt cs skE pkR info aad pt =
-  let pkE, keyIR, nonceIR = encap cs skE pkR info in
-  let ct = AEAD.aead_encrypt (aead_of_cs cs) keyIR nonceIR pt aad in
-  ct, pkE
+let setupBaseI cs skE pkR info =
+  let zz, pkE = encap cs skE pkR in
+  let k,n = ks_derive cs Base pkR zz pkE info None None in
+  pkE, k, n
 
 
-/// Decrypt()
-///
-/// Input: ciphersuite, skR, pkE, info, ad, ct
-///
-///    1. keyIR, nonceIR = Decap(ciphersuite, pkE, pkR, info)
-///    2. pt = Open(keyIR, nonceIR, ad, ct)
-///
-/// Output: pt
+/// def SetupBaseR(enc, skR, info):
+///     zz = Decap(enc, skR)
+///     return KeySchedule(mode_base, pk(skR), zz, enc, info,
+///                        default_psk, default_pskID, default_pkIm)
 
-val decrypt:
-    cs: ciphersuite
-  -> skR: key_dh_secret_s cs
+val setupBaseR:
+    cs:ciphersuite
   -> pkE: key_dh_public_s cs
-  -> info: lbytes size_einfo
-  -> aad: bytes{length aad + AEAD.padlen (aead_of_cs cs) (length aad) <= max_size_t}
-  -> ct: bytes{AEAD.size_tag (aead_of_cs cs) <= length ct
-             /\ (length ct + length aad) / 64 <= max_size_t
-             /\ length ct + AEAD.size_block (aead_of_cs cs) <= max_size_t}
-  -> mac: AEAD.tag (aead_of_cs cs) ->
-  Tot (option (lbytes (length ct)))
+  -> skR:key_dh_secret_s cs
+  -> info:bytes{Seq.length info <= max_info} ->
+  Tot (key_aead_s cs & nonce_aead_s cs)
 
-let decrypt cs skR pkE info aad ct mac =
-  let keyIR, nonceIR = decap cs pkE skR info in
-  AEAD.aead_decrypt (aead_of_cs cs) keyIR nonceIR ct mac aad
+let setupBaseR cs pkE skR info =
+  let pkR = DH.secret_to_public (curve_of_cs cs) skR in
+  let zz = decap cs pkE skR in
+  ks_derive cs Base pkR zz pkE info None None
+
+
+/// def SetupAuthI(pkR, skI, info):
+///     zz, enc = AuthEncap(pkR, skI)
+///     pkIm = Marshal(pk(skI))
+///     return enc, KeySchedule(pkR, zz, enc, info,
+///                             default_psk, default_pskID, pkIm)
+
+val setupAuthI:
+    cs:ciphersuite
+  -> skE: key_dh_secret_s cs
+  -> skI: key_dh_secret_s cs
+  -> pkR:key_dh_public_s cs
+  -> info:bytes{Seq.length info <= max_info} ->
+  Tot (key_dh_public_s cs & key_aead_s cs & nonce_aead_s cs)
+
+let setupAuthI cs skE skI pkR info =
+  let pkI = DH.secret_to_public (curve_of_cs cs) skI in
+  let zz, pkE = auth_encap cs skE skI pkR in
+  let k, n = ks_derive cs Auth pkR zz pkE info None (Some pkI) in
+  pkE, k, n
+
+
+/// def SetupAuthR(enc, skR, pkI, info):
+///     zz = AuthDecap(enc, skR, pkI)
+///     pkIm = Marshal(pkI)
+///     return KeySchedule(pk(skR), zz, enc, info,
+///                        default_psk, default_pskID, pkIm)
+
+val setupAuthR:
+    cs:ciphersuite
+  -> pkE: key_dh_public_s cs
+  -> pkI: key_dh_public_s cs
+  -> skR:key_dh_secret_s cs
+  -> info:bytes{Seq.length info <= max_info} ->
+  Tot (key_aead_s cs & nonce_aead_s cs)
+
+let setupAuthR cs pkE pkI skR info =
+  let pkR = DH.secret_to_public (curve_of_cs cs) skR in
+  let zz = auth_decap cs pkE pkI skR in
+  ks_derive cs Auth pkR zz pkE info None (Some pkI)
+
+
+/// def SetupAuthI(pkR, psk, pskID, skI, info):
+///     zz, enc = AuthEncap(pkR, skI)
+///     pkIm = Marshal(pk(skI))
+///     return enc, KeySchedule(pkR, zz, enc, info, psk, pskID, pkIm)
+
+val setupPSKAuthI:
+    cs:ciphersuite
+  -> skE: key_dh_secret_s cs
+  -> skI: key_dh_secret_s cs
+  -> pkR: key_dh_public_s cs
+  -> psk: psk_s cs
+  -> pskID: bytes{Seq.length pskID <= max_pskID}
+  -> info:bytes{Seq.length info <= max_info} ->
+  Tot (key_dh_public_s cs & key_aead_s cs & nonce_aead_s cs)
+
+let setupPSKAuthI cs skE skI pkR psk pskID info =
+  let pkI = DH.secret_to_public (curve_of_cs cs) skI in
+  let zz, pkE = auth_encap cs skE skI pkR in
+  let k, n = ks_derive cs PSKAuth pkR zz pkE info (Some (psk, pskID)) (Some pkI) in
+  pkE, k, n
+
+
+/// def SetupAuthR(enc, skR, psk, pskID, pkI, info):
+///     zz = AuthDecap(enc, skR, pkI)
+///     pkIm = Marshal(pkI)
+///     return KeySchedule(pk(skR), zz, enc, info, psk, pskID, pkIm)
+
+val setupPSKAuthR:
+    cs:ciphersuite
+  -> pkE: key_dh_public_s cs
+  -> pkI: key_dh_public_s cs
+  -> skR:key_dh_secret_s cs
+  -> psk: psk_s cs
+  -> pskID: bytes{Seq.length pskID <= max_pskID}
+  -> info:bytes{Seq.length info <= max_info} ->
+  Tot (key_aead_s cs & nonce_aead_s cs)
+
+let setupPSKAuthR cs pkE pkI skR psk pskID info =
+  let pkR = DH.secret_to_public (curve_of_cs cs) skR in
+  let zz = auth_decap cs pkE pkI skR in
+  ks_derive cs PSKAuth pkR zz pkE info (Some (psk, pskID)) (Some pkI)
+
+
+/// Encrypt() and Decrypt using the derived AEAD key and nonce
+/// are implemented by calling AEAD.encrypt and AEAD.Decrypt
